

# Assignment 5 Solutions

MA6.102 Probability and Random Processes, Monsoon 2025

## Question 1

Given:

$$f_{X,Y}(x, y) = c \cdot x(y - x)e^{-y}, \quad 0 \leq x \leq y < \infty$$

We need to find  $c$  such that:

$$\int_0^\infty \int_0^y c \cdot x(y - x)e^{-y} dx dy = 1$$

First, evaluate the inner integral:

$$\begin{aligned} \int_0^y x(y - x) dx &= \int_0^y (xy - x^2) dx = y \int_0^y x dx - \int_0^y x^2 dx \\ &= y \left[ \frac{x^2}{2} \right]_0^y - \left[ \frac{x^3}{3} \right]_0^y = \frac{y^3}{2} - \frac{y^3}{3} = \frac{y^3}{6} \end{aligned}$$

Therefore:

$$\frac{c}{6} \int_0^\infty y^3 e^{-y} dy = 1$$

Now evaluate  $\int_0^\infty y^3 e^{-y} dy$  using integration by parts:

$$\begin{aligned} \int_0^\infty y^3 e^{-y} dy &= [-y^3 e^{-y}]_0^\infty + 3 \int_0^\infty y^2 e^{-y} dy = 3 \int_0^\infty y^2 e^{-y} dy \\ &= 3 \left( [-y^2 e^{-y}]_0^\infty + 2 \int_0^\infty y e^{-y} dy \right) = 6 \int_0^\infty y e^{-y} dy \\ &= 6 \left( [-y e^{-y}]_0^\infty + \int_0^\infty e^{-y} dy \right) = 6(0 + 1) = 6 \end{aligned}$$

Thus,  $c = 1$ .

The marginal density of  $Y$  is:

$$f_Y(y) = \int_0^y x(y - x)e^{-y} dx = e^{-y} \cdot \frac{y^3}{6}, \quad y \geq 0$$

The conditional density is:

$$f_{X|Y}(x | y) = \frac{f_{X,Y}(x, y)}{f_Y(y)} = \frac{x(y - x)e^{-y}}{(y^3/6)e^{-y}} = \frac{6x(y - x)}{y^3}, \quad 0 \leq x \leq y$$

The conditional expectation is:

$$\begin{aligned} E[X \mid Y = y] &= \int_0^y x \cdot f_{X|Y}(x \mid y) dx = \frac{6}{y^3} \int_0^y x^2(y-x) dx \\ &= \frac{6}{y^3} \left( y \int_0^y x^2 dx - \int_0^y x^3 dx \right) = \frac{6}{y^3} \left( y \cdot \frac{y^3}{3} - \frac{y^4}{4} \right) \\ &= \frac{6}{y^3} \left( \frac{y^4}{3} - \frac{y^4}{4} \right) = \frac{6}{y^3} \cdot \frac{y^4}{12} = \frac{y}{2} \end{aligned}$$

Therefore:

$$E[X \mid Y] = \frac{Y}{2}$$

## Question 2

Let  $X_1$  and  $X_2$  be independent and identically distributed random variables with the common PDF  $f_X(x) = \frac{1}{x^2}$ , for  $x > 1$ . Define new random variables  $Y_1 = X_1 + X_2$  and  $Y_2 = \frac{X_2}{X_1 + X_2}$ . Find the joint PDF, explicitly stating the domain over which it is non-zero.

### Solution

We will use the method of Jacobian transformation. For this, we need the joint density of  $X_1$  and  $X_2$ , and the Jacobian determinant itself.

Since  $X_1$  and  $X_2$  are independent, their joint PDF is the product of the marginal PDFs:

$$f_{X_1, X_2}(x_1, x_2) = f_{X_1}(x_1) \cdot f_{X_2}(x_2)$$

Given  $f_X(x) = \frac{1}{x^2}$  for  $x > 1$ , we have:

$$f_{X_1, X_2}(x_1, x_2) = \left(\frac{1}{x_1^2}\right) \left(\frac{1}{x_2^2}\right) = \frac{1}{x_1^2 x_2^2}$$

This joint PDF is non-zero on the domain  $D_X = \{(x_1, x_2) : x_1 > 1, x_2 > 1\}$ .

We are given the transformations:

$$\begin{aligned} Y_1 &= X_1 + X_2 \\ Y_2 &= \frac{X_2}{X_1 + X_2} \end{aligned}$$

We now solve for  $x_1$  and  $x_2$  in terms of  $y_1$  and  $y_2$ . From the definition of  $Y_2$ :

$$Y_2 = \frac{X_2}{Y_1} \Rightarrow X_2 = Y_1 Y_2$$

From the definition of  $Y_1$ :

$$X_1 = Y_1 - X_2 = Y_1 - Y_1 Y_2 = Y_1(1 - Y_2)$$

The inverse transformations are:

$$\begin{aligned} x_1 &= y_1(1 - y_2) \\ x_2 &= y_1 y_2 \end{aligned}$$

Finding the Jacobian  $J$ :

We compute the Jacobian with respect to  $x_1$  and  $x_2$ :  $J = \det \begin{vmatrix} \frac{\partial y_1}{\partial x_1} & \frac{\partial y_1}{\partial x_2} \\ \frac{\partial y_2}{\partial x_1} & \frac{\partial y_2}{\partial x_2} \end{vmatrix}$

From the transformations  $y_1 = x_1 + x_2$  and  $y_2 = \frac{x_2}{x_1 + x_2}$ :

$$\begin{aligned} \frac{\partial y_1}{\partial x_1} &= 1, & \frac{\partial y_1}{\partial x_2} &= 1 \\ \frac{\partial y_2}{\partial x_1} &= -\frac{x_2}{(x_1 + x_2)^2}, & \frac{\partial y_2}{\partial x_2} &= \frac{x_1}{(x_1 + x_2)^2} \end{aligned}$$

The determinant is:  $J = (1) \left(\frac{x_1}{(x_1 + x_2)^2}\right) - (1) \left(-\frac{x_2}{(x_1 + x_2)^2}\right) = \frac{x_1 + x_2}{(x_1 + x_2)^2} = \frac{1}{x_1 + x_2}$

Since  $x_1 + x_2 = y_1$ , we have  $|J| = \frac{1}{y_1}$ .

The formula for the joint PDF using this Jacobian is:  $f_{Y_1, Y_2}(y_1, y_2) = \frac{f_{X_1, X_2}(x_1(y_1, y_2), x_2(y_1, y_2))}{|J|}$

**Alternative Method:** We can also compute the Jacobian with respect to  $y_1$  and  $y_2$ :

$$J' = \det \begin{vmatrix} \frac{\partial x_1}{\partial y_1} & \frac{\partial x_1}{\partial y_2} \\ \frac{\partial x_2}{\partial y_1} & \frac{\partial x_2}{\partial y_2} \end{vmatrix}$$

Computing the partial derivatives:

$$\begin{aligned} \frac{\partial x_1}{\partial y_1} &= 1 - y_2, & \frac{\partial x_1}{\partial y_2} &= -y_1 \\ \frac{\partial x_2}{\partial y_1} &= y_2, & \frac{\partial x_2}{\partial y_2} &= y_1 \end{aligned}$$

The determinant is:  $J' = (1 - y_2)(y_1) - (-y_1)(y_2) = y_1 - y_1 y_2 + y_1 y_2 = y_1$

Note that  $J' = \frac{1}{J}$ , so  $|J'| = y_1$ , and the transformation formula becomes:  $f_{Y_1, Y_2}(y_1, y_2) = f_{X_1, X_2}(x_1(y_1, y_2), x_2(y_1, y_2)) \cdot |J'|$

Both methods give the same result.

We map the original domain  $D_X$  to the new domain  $D_Y$  using the inverse transformation. The original domain  $D_X$  is defined by two conditions:  $x_1 > 1$  and  $x_2 > 1$ .

Substituting the inverse functions into these inequalities:

1.  $y_1(1 - y_2) > 1$
2.  $y_1 y_2 > 1$

These two inequalities define the domain  $D_Y$  where the joint PDF of  $Y$  is non-zero. (We can also deduce that  $y_1 > 2$ ,  $0 < y_2 < 1$ , and  $y_1 > \max\left(\frac{1}{y_2}, \frac{1}{1-y_2}\right)$ ).

The formula for the joint PDF of the new variables is:  $f_{Y_1, Y_2}(y_1, y_2) = \frac{f_{X_1, X_2}(x_1(y_1, y_2), x_2(y_1, y_2))}{|J|}$

Substituting  $x_1 = y_1(1 - y_2)$  and  $x_2 = y_1 y_2$ :  $f_{Y_1, Y_2}(y_1, y_2) = \frac{1}{[y_1(1-y_2)]^2 [y_1 y_2]^2} \cdot y_1 = \frac{y_1}{y_1^4 y_2^2 (1-y_2)^2}$

$$f_{Y_1, Y_2}(y_1, y_2) = \frac{1}{y_1^3 y_2^2 (1 - y_2)^2}$$

This PDF is non-zero on the domain  $D_Y$ :

$$D_Y = \{(y_1, y_2) : y_1 y_2 > 1 \text{ and } y_1(1 - y_2) > 1\}$$

**Final Answer:**

$$f_{Y_1, Y_2}(y_1, y_2) = \frac{1}{y_1^3 y_2^2 (1 - y_2)^2}$$

for the domain:

$$y_1 y_2 > 1 \text{ and } y_1(1 - y_2) > 1$$

and  $f_{Y_1, Y_2}(y_1, y_2) = 0$  elsewhere.

### Problem 3

Let  $X_1$  and  $X_2$  be independent exponential random variables with parameter  $\lambda$ . Find the joint PDF of

$$Y_1 = X_1 + X_2, \quad Y_2 = \frac{X_1}{X_2},$$

and check whether  $Y_1$  and  $Y_2$  are independent.

$$f_{X_1, X_2}(x_1, x_2) = \begin{cases} \lambda^2 e^{-\lambda(x_1 + x_2)}, & x_1 > 0, x_2 > 0, \\ 0, & \text{otherwise.} \end{cases}$$

$$Y_1 = X_1 + X_2, \quad Y_2 = \frac{X_1}{X_2}$$

$$X_1 = Y_1 \frac{Y_2}{1 + Y_2}, \quad X_2 = \frac{Y_1}{1 + Y_2}$$

Support:  $y_1 > 0, y_2 > 0$ .

#### Method 1

$$J_1 = \det \left( \frac{\partial(x_1, x_2)}{\partial(y_1, y_2)} \right) = \begin{vmatrix} \frac{\partial x_1}{\partial y_1} & \frac{\partial x_1}{\partial y_2} \\ \frac{\partial x_2}{\partial y_1} & \frac{\partial x_2}{\partial y_2} \end{vmatrix} = \begin{vmatrix} \frac{y_2}{1 + y_2} & \frac{y_1}{(1 + y_2)^2} \\ \frac{1}{1 + y_2} & -\frac{y_1}{(1 + y_2)^2} \end{vmatrix}$$

$$= \left( \frac{y_2}{1 + y_2} \right) \left( -\frac{y_1}{(1 + y_2)^2} \right) - \left( \frac{y_1}{(1 + y_2)^2} \right) \left( \frac{1}{1 + y_2} \right)$$

$$= -\frac{y_1(y_2 + 1)}{(1 + y_2)^3} = -\frac{y_1}{(1 + y_2)^2}$$

$$|J_1| = \frac{y_1}{(1 + y_2)^2}$$

$$\begin{aligned} f_{Y_1, Y_2}(y_1, y_2) &= f_{X_1, X_2}(x_1, x_2) |J_1| = \lambda^2 e^{-\lambda(x_1 + x_2)} \frac{y_1}{(1 + y_2)^2} \\ &= \lambda^2 e^{-\lambda y_1} \frac{y_1}{(1 + y_2)^2} = \lambda^2 y_1 e^{-\lambda y_1} (1 + y_2)^{-2} \end{aligned}$$

## Method 2

$$\begin{aligned}
J_2 &= \det \left( \frac{\partial(y_1, y_2)}{\partial(x_1, x_2)} \right) = \begin{vmatrix} \frac{\partial y_1}{\partial x_1} & \frac{\partial y_1}{\partial x_2} \\ \frac{\partial y_2}{\partial x_1} & \frac{\partial y_2}{\partial x_2} \end{vmatrix} = \begin{vmatrix} 1 & 1 \\ \frac{1}{x_2} & -\frac{x_1}{x_2^2} \end{vmatrix} \\
&= (1) \left( -\frac{x_1}{x_2^2} \right) - (1) \left( \frac{1}{x_2} \right) = -\frac{x_1 + x_2}{x_2^2} \\
|J_2| &= \frac{x_1 + x_2}{x_2^2} \\
f_{Y_1, Y_2}(y_1, y_2) &= \frac{f_{X_1, X_2}(x_1, x_2)}{|J_2|} = \frac{\lambda^2 e^{-\lambda(x_1 + x_2)}}{\left( \frac{x_1 + x_2}{x_2^2} \right)} = \lambda^2 e^{-\lambda(x_1 + x_2)} \left( \frac{x_2^2}{x_1 + x_2} \right) \\
&= \lambda^2 e^{-\lambda y_1} \left( \frac{\left( \frac{y_1}{1 + y_2} \right)^2}{y_1} \right) = \lambda^2 e^{-\lambda y_1} \left( \frac{y_1^2 / (1 + y_2)^2}{y_1} \right) \\
&= \lambda^2 e^{-\lambda y_1} \left( \frac{y_1}{(1 + y_2)^2} \right) = \lambda^2 y_1 e^{-\lambda y_1} (1 + y_2)^{-2}
\end{aligned}$$


---

$$f_{Y_1, Y_2}(y_1, y_2) = \begin{cases} \lambda^2 y_1 e^{-\lambda y_1} (1 + y_2)^{-2}, & y_1 > 0, y_2 > 0, \\ 0, & \text{otherwise.} \end{cases}$$

$$\begin{aligned}
f_{Y_1}(y_1) &= \int_0^\infty \lambda^2 y_1 e^{-\lambda y_1} (1 + y_2)^{-2} dy_2 \\
&= \lambda^2 y_1 e^{-\lambda y_1} \int_0^\infty (1 + y_2)^{-2} dy_2 \\
&= \lambda^2 y_1 e^{-\lambda y_1} \left[ -(1 + y_2)^{-1} \right]_0^\infty = \lambda^2 y_1 e^{-\lambda y_1}, \quad y_1 > 0.
\end{aligned}$$

$$\begin{aligned}
f_{Y_2}(y_2) &= \int_0^\infty \lambda^2 y_1 e^{-\lambda y_1} (1 + y_2)^{-2} dy_1 \\
&= (1 + y_2)^{-2} \int_0^\infty \lambda^2 y_1 e^{-\lambda y_1} dy_1 \\
&= (1 + y_2)^{-2} \cdot 1 = (1 + y_2)^{-2}, \quad y_2 > 0.
\end{aligned}$$

$$f_{Y_1}(y_1) f_{Y_2}(y_2) = (\lambda^2 y_1 e^{-\lambda y_1}) \cdot ((1 + y_2)^{-2}) = f_{Y_1, Y_2}(y_1, y_2).$$

Therefore,  $Y_1$  and  $Y_2$  are independent.

### Problem 5.

$$X, Y, Z \stackrel{\text{iid}}{\sim} \text{Unif}(0, 1), \quad W = XY.$$

$$\begin{aligned} F_W(w) &= P(XY \leq w) = \int_0^1 P\left(X \leq \frac{w}{y}\right) dy \\ &= \int_0^1 \min\left(1, \frac{w}{y}\right) dy = \int_0^w 1 dy + \int_w^1 \frac{w}{y} dy \\ &= w + w \ln\left(\frac{1}{w}\right) = w - w \ln w, \quad 0 < w \leq 1, \end{aligned}$$

$$f_W(w) = F'_W(w) = -\ln w, \quad 0 < w < 1.$$

$$\begin{aligned} P(XY < Z^2) &= \iint_{[0,1]^2} \mathbf{1}_{\{w < z^2\}} f_W(w) f_Z(z) dw dz \\ &= \int_0^1 f_W(w) P(Z > \sqrt{w}) dw \\ &= \int_0^1 (-\ln w) (1 - \sqrt{w}) dw \\ &= \int_0^1 (-\ln w) dw - \int_0^1 (-\ln w) \sqrt{w} dw. \end{aligned}$$

$$\int_0^1 (-\ln w) dw = 1, \quad \int_0^1 (-\ln w) \sqrt{w} dw = - \int_0^1 w^{1/2} \ln w dw = \frac{4}{9}.$$

$$P(XY < Z^2) = 1 - \frac{4}{9} = \frac{5}{9}.$$

$$\boxed{P(XY < Z^2) = \frac{5}{9}.}$$

## Question 6

Let  $F_X$  and  $F_Y$  be strictly increasing CDFs of random variables  $X$  and  $Y$ . Since they are strictly increasing, the ordinary inverses  $F_X^{-1}$  and  $F_Y^{-1}$  exist on  $(0, 1)$ . Define

$$g(x) = F_Y^{-1}(F_X(x)), \quad Z = g(X).$$

We prove  $F_Z(y) = F_Y(y)$  by starting from  $F_Y(y)$ :

$$\begin{aligned} F_Y(y) &= F_X(F_X^{-1}(F_Y(y))) && \text{(inverse identity)} \\ &= \mathbb{P}\{X \leq F_X^{-1}(F_Y(y))\} && \text{(definition of } F_X) \\ &= \mathbb{P}\{F_X(X) \leq F_Y(y)\} && \text{(apply increasing } F_X \text{ to both sides)} \\ &= \mathbb{P}\{F_Y^{-1}(F_X(X)) \leq y\} && \text{(apply increasing } F_Y^{-1} \text{ to both sides)} \\ &= \mathbb{P}\{Z \leq y\} && \text{(since } Z = F_Y^{-1}(F_X(X))) \\ &= F_Z(y). \end{aligned}$$

Thus  $Z = g(X)$  has the same CDF as  $Y$ .



## Question 7

(a)

Yes, the statement is **true**.

The characteristic function is defined as  $\phi_X(t) = \mathbb{E}[e^{itX}]$ . We are given the condition  $\phi_X(2\pi) = 1$ . By definition, this means  $\mathbb{E}[e^{i2\pi X}] = 1$ . Using Euler's formula,  $e^{i\theta} = \cos(\theta) + i\sin(\theta)$ , we can expand the expectation:

$$\mathbb{E}[\cos(2\pi X) + i\sin(2\pi X)] = 1$$

By the linearity of expectation, this separates into real and imaginary parts:

$$\mathbb{E}[\cos(2\pi X)] + i\mathbb{E}[\sin(2\pi X)] = 1 + 0i$$

Equating the real and imaginary parts, we get two conditions:

$$\mathbb{E}[\cos(2\pi X)] = 1$$

$$\mathbb{E}[\sin(2\pi X)] = 0$$

Let's focus on the first condition. The cosine function has a maximum value of 1, so  $\cos(2\pi X) \leq 1$  for all outcomes of  $X$ . If the expected value of a random variable is equal to its maximum possible value, the random variable must equal that maximum value with probability 1.

Therefore, we must have  $\mathbb{P}(\cos(2\pi X) = 1) = 1$ . The equation  $\cos(\theta) = 1$  holds if and only if  $\theta = 2\pi k$  for some integer  $k \in \mathbb{Z}$ . Applying this to our case:

$$2\pi X = 2\pi k \implies X = k \quad \text{for some } k \in \mathbb{Z}$$

This means the random variable  $X$  must take an integer value with probability 1. Thus, we have shown that  $\mathbb{P}(X \in \mathbb{Z}) = 1$ . Note that the second expectation condition is also satisfied.

(b)

We want to show that  $P_X(n) = \frac{1}{2\pi} \int_0^{2\pi} e^{-itn} \phi_X(t) dt$ .

For an integer-valued random variable  $X$ , the characteristic function is given by the sum over all possible integer outcomes  $k$ :

$$\phi_X(t) = \mathbb{E}[e^{itX}] = \sum_{k \in \mathbb{Z}} e^{itk} P_X(k)$$

We start with the right-hand side (RHS) of the equation to be proved and substitute this definition.

$$\begin{aligned} \text{RHS} &= \frac{1}{2\pi} \int_0^{2\pi} e^{-itn} \phi_X(t) dt \\ &= \frac{1}{2\pi} \int_0^{2\pi} e^{-itn} \left( \sum_{k \in \mathbb{Z}} e^{itk} P_X(k) \right) dt \end{aligned}$$

We interchange the order of integration and summation:

$$\begin{aligned} \text{RHS} &= \frac{1}{2\pi} \sum_{k \in \mathbb{Z}} P_X(k) \int_0^{2\pi} e^{-itn} e^{itk} dt \\ &= \frac{1}{2\pi} \sum_{k \in \mathbb{Z}} P_X(k) \int_0^{2\pi} e^{it(k-n)} dt \end{aligned}$$

Now, we evaluate the integral  $\int_0^{2\pi} e^{it(k-n)} dt$  based on two cases for the integers  $k$  and  $n$ .

- **Case 1:**  $k = n$ . The exponent is 0, so the integrand is  $e^0 = 1$ .

$$\int_0^{2\pi} 1 dt = [t]_0^{2\pi} = 2\pi$$

- **Case 2:**  $k \neq n$ . The integral evaluates to:

$$\int_0^{2\pi} e^{it(k-n)} dt = \left[ \frac{e^{it(k-n)}}{i(k-n)} \right]_0^{2\pi} = \frac{e^{i2\pi(k-n)} - e^0}{i(k-n)}$$

Since  $k - n$  is a non-zero integer,  $e^{i2\pi(k-n)} = 1$ . Thus, the integral is  $\frac{1-1}{i(k-n)} = 0$ .

So, the integral is non-zero only when  $k = n$ . This causes the infinite sum to collapse to a single term.

$$\begin{aligned} \text{RHS} &= \frac{1}{2\pi} \sum_{k \in \mathbb{Z}} P_X(k) \cdot \begin{cases} 2\pi & \text{if } k = n \\ 0 & \text{if } k \neq n \end{cases} \\ &= \frac{1}{2\pi} (P_X(n) \cdot 2\pi) \\ &= P_X(n) \end{aligned}$$

The right-hand side equals the left-hand side, which completes the proof.

## Problem 4

### Given Formula

Let  $(X, Y)$  be jointly continuous with joint pdf  $f_{X,Y}(x, y)$ . Let

$$Z = g_1(X, Y), \quad W = g_2(X, Y),$$

$$g_1(x, y) = z, \quad g_2(x, y) = w$$

$(x_i, y_i)$ ,  $i = 1, \dots, n$ . Define

$$J(x_i, y_i) = \left| \det \begin{pmatrix} \frac{\partial g_1(x, y)}{\partial x} & \frac{\partial g_1(x, y)}{\partial y} \\ \frac{\partial g_2(x, y)}{\partial x} & \frac{\partial g_2(x, y)}{\partial y} \end{pmatrix} \right|_{(x, y) = (x_i, y_i)}.$$

Then the joint pdf of  $(Z, W)$  is

$$f_{Z,W}(z, w) = \sum_{i=1}^n \frac{f_{X,Y}(x_i, y_i)}{J(x_i, y_i)}.$$

**Apply to**  $Z = \min\{X, Y\}$ ,  $W = \max\{X, Y\}$

We take

$$g_1(x, y) = \min\{x, y\}, \quad g_2(x, y) = \max\{x, y\}.$$

**Solve**  $g_1(x, y) = z$ ,  $g_2(x, y) = w$

Fix  $(z, w)$  with  $z < w$ . The equations

$$\min\{x, y\} = z, \quad \max\{x, y\} = w$$

have exactly two solutions:

$$(x_1, y_1) = (z, w), \quad (x_2, y_2) = (w, z).$$

### Compute $J$ at each region

- $(x_1, y_1) = (z, w)$  with  $z < w$ : Therefore

$$J(x_1, y_1) = \left| \det \begin{pmatrix} 1 & 0 \\ 0 & 1 \end{pmatrix} \right| = 1.$$

### Reason

$$\begin{aligned} \frac{\partial z}{\partial x}(z, w) &= \lim_{h \rightarrow 0} \frac{z(z+h, w) - z(z, w)}{h} = \lim_{h \rightarrow 0} \frac{\min(z+h, w) - \min(z, w)}{h} \\ &= \lim_{h \rightarrow 0} \frac{(z+h) - z}{h} = 1, \end{aligned}$$

$$\begin{aligned} \frac{\partial z}{\partial y}(z, w) &= \lim_{h \rightarrow 0} \frac{z(z, w+h) - z(z, w)}{h} = \lim_{h \rightarrow 0} \frac{\min(z, w+h) - \min(z, w)}{h} \\ &= \lim_{h \rightarrow 0} \frac{z - z}{h} = 0, \end{aligned}$$

$$\begin{aligned} \frac{\partial w}{\partial x}(z, w) &= \lim_{h \rightarrow 0} \frac{w(z+h, w) - w(z, w)}{h} = \lim_{h \rightarrow 0} \frac{\max(z+h, w) - \max(z, w)}{h} \\ &= \lim_{h \rightarrow 0} \frac{w - w}{h} = 0, \end{aligned}$$

$$\begin{aligned} \frac{\partial w}{\partial y}(z, w) &= \lim_{h \rightarrow 0} \frac{w(z, w+h) - w(z, w)}{h} = \lim_{h \rightarrow 0} \frac{\max(z, w+h) - \max(z, w)}{h} \\ &= \lim_{h \rightarrow 0} \frac{(w+h) - w}{h} = 1. \end{aligned}$$

$$J(z, w) = \begin{pmatrix} \frac{\partial z}{\partial x} & \frac{\partial z}{\partial y} \\ \frac{\partial w}{\partial x} & \frac{\partial w}{\partial y} \end{pmatrix} = \begin{pmatrix} 1 & 0 \\ 0 & 1 \end{pmatrix}, \quad |\det J(z, w)| = 1.$$

- $(x_2, y_2) = (w, z)$  with  $w > z$ : Therefore

$$J(x_2, y_2) = \left| \det \begin{pmatrix} 0 & 1 \\ 1 & 0 \end{pmatrix} \right| = 1.$$

### Plugging into formula

$$f_{Z,W}(z, w) = \frac{f_{X,Y}(x_1, y_1)}{J(x_1, y_1)} + \frac{f_{X,Y}(x_2, y_2)}{J(x_2, y_2)} = f_{X,Y}(z, w) + f_{X,Y}(w, z), \quad (z < w).$$

Since  $Z = \min\{X, Y\} \leq W = \max\{X, Y\}$  by definition,

$$f_{Z,W}(z, w) = \begin{cases} f_{X,Y}(z, w) + f_{X,Y}(w, z), & z \leq w, \end{cases}$$